working on cleaning up symbolic evaluation.

src/SymEval.v
@@ -8,11 +8,14 @@ Require Import Env.
 Set Implicit Arguments.
 Set Strict Implicit.
 
-Module MemoryEvaluator (SH : SepHeap).
+Module SymbolicEvaluator (SH : SepHeap).
   Module SEP := SH.SE.
   Module ST := SEP.ST.
 
-  (** Learn hook **)
+  (** Learn hook
+   ** - This is the bit of code that gets run with new pure facts are
+   **   learned during symbolic evaluation
+   **)
   Section LearnHook.
     Variable types_ : list type.
     Variable SymState : Type.
@@ -55,14 +58,18 @@ Module MemoryEvaluator (SH : SepHeap).
       end.
   End LearnHookDefault.
 
+  (** Memory Evaluator
+   ** - This is the bit of code that gets run when we try to read
+   **   or write to memory.
+   **)
   Section MemEvaluator.
     Variable types : list type.
     Variables pcT stT : tvar.
 
     Record MemEvaluator : Type :=
-    { smemeval_read_word : forall (P : ProverT types), Facts P -> 
+    { sread_word : forall (P : ProverT types), Facts P -> 
       expr types -> SH.SHeap types pcT stT -> option (expr types)
-    ; smemeval_write_word : forall (P : ProverT types), Facts P ->
+    ; swrite_word : forall (P : ProverT types), Facts P ->
       expr types -> expr types -> SH.SHeap types pcT stT -> option (SH.SHeap types pcT stT)
     }.
 
@@ -83,7 +90,7 @@ Module MemoryEvaluator (SH : SepHeap).
     { ReadCorrect :
       forall (P : ProverT types) (PE : ProverT_correct P funcs),
         forall facts pe ve SH,
-          smemeval_read_word eval P facts pe SH = Some ve ->
+          sread_word eval P facts pe SH = Some ve ->
           forall uvars vars cs p stn_m,
             Valid PE uvars vars facts ->
             exprD funcs uvars vars pe ptrT = Some p ->
@@ -96,7 +103,7 @@ Module MemoryEvaluator (SH : SepHeap).
     ; WriteCorrect :
       forall (P : ProverT types) (PE : ProverT_correct P funcs),
         forall uvars vars cs facts pe ve SH SH',
-          smemeval_write_word eval P facts pe ve SH = Some SH' ->
+          swrite_word eval P facts pe ve SH = Some SH' ->
           Valid PE uvars vars facts ->
           forall p v,
             exprD funcs uvars vars pe ptrT = Some p ->
@@ -174,30 +181,28 @@ Module MemoryEvaluator (SH : SepHeap).
 
   End Default.
 
-  (** Plugins are symbolic evaluators that handle single predicates **)
-  Module Plugin.
-    Module SEP := SEP.
+  (** Evaluators for single predicates
+   ** - this abstracts the common case when we are considering
+   **   a single predicate in isolation
+   ** - TODO: I do not know how to make symbolic memory work with 
+   **   this definition. I want to use the predicates in SepTheoryX
+   **   but there is no generic reading function & I can't specialize
+   **   until I know what [valT] refers to.
+   **)
+  Module PredEval.
+    Module SF := SepExpr.SepExprFacts SEP.
+
     Section typed.
       Variable types : list type.
 
       Record MemEvalPred : Type :=
-      { smem_read  : 
+      { pred_read_word  : 
         forall (P : ProverT types) (facts : Facts P) (args : exprs types) (p : expr types),
           option (expr types)
-      ; smem_write : 
+      ; pred_write_word : 
         forall (P : ProverT types) (facts : Facts P) (args : exprs types) (p v : expr types),
           option (exprs types)
       }.
-
-      Theorem proj_sym_read : forall a b,
-        smem_read (Build_MemEvalPred a b) = a.
-      Proof. reflexivity. Qed.
-      
-      Theorem proj_sym_write : forall a b,
-        smem_write (Build_MemEvalPred a b) = b.
-      Proof. reflexivity. Qed.
-
-      Variable me : MemEvalPred.
 
       Variables pcT stT : tvar.
 
@@ -208,12 +213,13 @@ Module MemoryEvaluator (SH : SepHeap).
       Hypothesis ReadWord : stn_st -> tvarD types ptrT -> option (tvarD types valT).
       Hypothesis WriteWord : stn_st -> tvarD types ptrT -> tvarD types valT -> option stn_st.
 
-      (** TODO: funcs should be removed from this? **)
-      Class MemEvalPred_correct (Predicate : SEP.ssignature types pcT stT)
+      Variable me : MemEvalPred.
+
+      Record MemEvalPred_correct (Predicate : SEP.ssignature types pcT stT)
         (funcs : functions types) : Prop :=
-      { sym_read_correct : forall P (PE : ProverT_correct P funcs),
+      { sym_read_word_correct : forall P (PE : ProverT_correct P funcs),
         forall args uvars vars cs facts pe p ve stn_st Q,
-          smem_read me P facts args pe = Some ve ->
+          pred_read_word me P facts args pe = Some ve ->
           Valid PE uvars vars facts ->
           exprD funcs uvars vars pe ptrT = Some p ->
           match 
@@ -227,9 +233,9 @@ Module MemoryEvaluator (SH : SepHeap).
               ReadWord stn_st p = Some v
             | _ => False
           end
-       ; sym_write_correct : forall P (PE : ProverT_correct P funcs),
+       ; sym_write_word_correct : forall P (PE : ProverT_correct P funcs),
          forall args uvars vars cs facts pe p ve v stn_st args' Q,
-           smem_write me P facts args pe ve = Some args' ->
+           pred_write_word me P facts args pe ve = Some args' ->
            Valid PE uvars vars facts ->
            exprD funcs uvars vars pe ptrT = Some p ->
            exprD funcs uvars vars ve valT = Some v ->
@@ -246,173 +252,294 @@ Module MemoryEvaluator (SH : SepHeap).
              | Some pr => 
                match WriteWord stn_st p v with
                  | None => False
-                 | Some sm' => mem_satisfies cs (ST.star pr Q) stn_st
+                 | Some sm' => mem_satisfies cs (ST.star pr Q) sm'
                end
            end
       }.
     End typed.
 
-    Section plugin.
+    Section search_read_write.
       Variable types : list type.
-      Variable pcT stT : tvar.
-      Variable evals : list (nat * MemEvalPred types). 
+      Variable T : Type.
+      Variable F : exprs types -> option T.
+      Variable F_upd : exprs types -> option (exprs types).
 
-      Section with_prover.
-        Variable Prover : ProverT types.
-
-        Section fold_first.
-          Variables T V : Type.
-          Variable F : T -> option V.
-
-          Fixpoint fold_first (ls : list T) : option V :=
-            match ls with
-              | nil => None
-              | t :: ls =>
-                match F t with
-                  | None => fold_first ls
-                  | x => x
-                end
-            end.
-        End fold_first.
-
-        Section fold_first_update.
-          Variable T : Type.
-          Variable F : T -> option T.
-
-          Fixpoint fold_first_update (ls : list T) (acc : list T) : option (list T) :=
-            match ls with
-              | nil => None
-              | t :: ls =>
-                match F t with
-                  | None => fold_first_update ls (t :: acc)
-                  | Some v => Some (rev acc ++ v :: ls)
-                end
-            end.
-        End fold_first_update.
-
-        Definition plugin_symeval_read_word (facts : Facts Prover) (p : expr types) 
-          (s : SH.SHeap types pcT stT) : option (expr types) :=
-          let impures := SH.impures s in
-          let reader i_me :=
-            let '(i,me) := i_me in
-            match FM.find i impures with
-              | Some argss =>
-                fold_first (fun args => smem_read me Prover facts args p) argss
-              | None => None
+      Fixpoint fold_args (es : list (exprs types)) : option T :=
+        match es with 
+          | nil => None
+          | a :: b => 
+            match F a with
+              | None => fold_args b
+              | Some r => Some r
             end
-          in
-          fold_first reader evals.
+        end.
+      
+      Theorem fold_args_correct : forall es v,
+        fold_args es = Some v ->
+        exists k, In k es /\ F k = Some v.
+      Proof.
+        clear. induction es.
+        simpl; congruence.
+        simpl. case_eq (F a); intros.
+        inversion H0. subst. eauto.
+        eapply IHes in H0. destruct H0.
+        exists x. tauto.
+      Qed.
 
-        Definition plugin_symeval_write_word (facts : Facts Prover) (p v : expr types)
-          (s : SH.SHeap types pcT stT) : option (SH.SHeap types pcT stT) :=
-          let impures := SH.impures s in
-          let writer i_me :=
-          let '(i,me) := i_me in
-            match FM.find i impures with
-              | Some argss =>
-                match fold_first_update (fun args => smem_write me Prover facts args p v) argss nil with
-                  | None => None
-                  | Some argss => Some (FM.add i argss impures) (** NOTE : add = replace **)
-                end
-              | None => None
+
+      Fixpoint fold_args_update (es : list (exprs types)) : option (list (exprs types)) :=
+        match es with 
+          | nil => None
+          | a :: b => 
+            match F_upd a with
+              | None => match fold_args_update b with
+                          | None => None
+                          | Some b => Some (a :: b)
+                        end
+              | Some r => Some (r :: b)
             end
-          in
-          match fold_first writer evals with
-            | None => None
-            | Some impures => Some (SH.Build_SHeap _ _ impures (SH.pures s) (SH.other s))
-          end.
-      End with_prover.
+        end.
+      
+      Theorem fold_args_update_correct : forall es es',
+        fold_args_update es = Some es' ->
+        exists pre, exists post, exists k, exists k',
+          es = pre ++ k :: post /\
+          F_upd k = Some k' /\
+          es' = pre ++ k' :: post.
+      Proof.
+        clear. induction es.
+        simpl; congruence.
+        simpl. case_eq (F_upd a); intros.
+        inversion H0. subst. do 4 eexists; intuition eauto.
+        instantiate (2 := nil). reflexivity. reflexivity.
 
-      Definition MemEvaluator_plugin : MemEvaluator types pcT stT : Type :=
-      {| smemeval_read_word := plugin_symeval_read_word
-       ; smemeval_write_word := plugin_symeval_write_word
-       |}.
-    End plugin.
+        generalize dependent H0.
+        case_eq (fold_args_update es); intros.
+        inversion H1; subst. eapply IHes in H0.
+        do 4 destruct H0. exists (a :: x). exists x0.
+        eexists; eexists; intuition; subst; eauto. reflexivity.
 
-    Section plugin_correct.
+        congruence.
+      Qed.
+
+    End search_read_write.
+
+    Section To_MemEvaluator.
       Variable types : list type.
-      Variables pcT stT : tvar.      
-      Variable evals : list (nat * MemEvalPred types).
+      Variables pcT stT : tvar.
+      
+      Variable mep : MemEvalPred types.
+      Variable predIndex : nat.
 
+      Definition MemEvalPred_to_MemEvaluator : MemEvaluator types pcT stT :=
+        {| sread_word := fun (P : ProverT types) (F : Facts P) (p : expr types) (h : SH.SHeap types pcT stT) =>
+           let impures := SH.impures h in
+           let argss := FM.find predIndex impures in
+           match argss with
+             | None => None
+             | Some argss => fold_args (fun args => @pred_read_word _ mep P F args p) argss
+           end
+         ; swrite_word := fun (P : ProverT types) (F : Facts P) (p v : expr types) (h : SH.SHeap types pcT stT) =>
+           let impures := SH.impures h in
+           let argss := FM.find predIndex impures in
+           match argss with
+             | None => None
+             | Some argss =>
+               match fold_args_update (fun args => @pred_write_word _ mep P F args p v) argss with
+                 | None => None
+                 | Some argss =>
+                   Some {| SH.impures := FM.add predIndex argss impures
+                         ; SH.pures   := SH.pures h
+                         ; SH.other   := SH.other h
+                         |}
+               end
+           end
+         |}.
+    
+      (** Correctness **)
       Variable funcs : functions types.
-      Variable sfuncs : SEP.predicates types pcT stT .
+      Variable preds : SEP.predicates types pcT stT.
 
       Variable stn_st : Type.
+    
       Variables ptrT valT : tvar.
 
-      Hypothesis mem_satisfies : PropX.codeSpec (tvarD types pcT) (tvarD types stT) -> 
-        ST.hprop (tvarD types pcT) (tvarD types stT) nil -> stn_st -> Prop.
+      Hypothesis mem_satisfies : PropX.codeSpec (tvarD types pcT) (tvarD types stT) -> ST.hprop (tvarD types pcT) (tvarD types stT) nil -> stn_st -> Prop.
       Hypothesis ReadWord : stn_st -> tvarD types ptrT -> option (tvarD types valT).
       Hypothesis WriteWord : stn_st -> tvarD types ptrT -> tvarD types valT -> option stn_st.
 
-      Fixpoint all T (P : T -> Prop) (ls : list T) : Prop :=
-        match ls with
-          | nil => True
-          | l :: ls => P l /\ all P ls
-        end.
+      Variable pred : SEP.ssignature types pcT stT.
+      Hypothesis predAt : nth_error preds predIndex = Some pred.
+      Hypothesis pred_correct :
+        @MemEvalPred_correct types pcT stT stn_st ptrT valT mem_satisfies ReadWord WriteWord mep pred funcs.
 
-      Definition ConsistentCondition : Prop := 
-        all (fun (i_me : nat * MemEvalPred types) => 
-          let (i,me) := i_me in
-            match nth_error sfuncs i with
-              | None => False
-              | Some s => @MemEvalPred_correct _ me pcT stT _ ptrT valT mem_satisfies ReadWord WriteWord s funcs
-            end) evals.
-        
-      Hypothesis sfuncs_evals : ConsistentCondition.
-
-      Definition PluginMemEvaluator_correct : 
-        @MemEvaluator_correct types _ _ (MemEvaluator_plugin pcT stT evals) funcs sfuncs _ _ _ mem_satisfies ReadWord WriteWord.
+      Lemma in_split : forall T (x : T) ls,
+        In x ls -> exists a b, ls = a ++ x :: b.
       Proof.
-        constructor; unfold ConsistentCondition in *; simpl.
-          (** read **)
-          unfold plugin_symeval_read_word. generalize dependent evals. clear.
-          induction evals; simpl; intros; try congruence ;
-            repeat match goal with
-                     | [ H : False |- _ ] => contradiction
-                     | [ H : prod _ _ |- _ ] => destruct H
-                     | [ H : context [ match FM.find ?A ?B with
-                                         | None => _ 
-                                         | Some _ => _ 
-                                       end ] |- _ ] => 
-                       revert H; case_eq (FM.find A B); intros
-                     | [ H : context [ match fold_first ?A ?B with
-                                         | None => _ 
-                                         | Some _ => _ 
-                                       end ] |- _ ] =>
-                     revert H; case_eq (fold_first A B); intros
-                     | [ H : context [ match nth_error ?A ?B with
-                                         | None => _ 
-                                         | Some _ => _ 
-                                       end ] |- _ ] =>
-                     revert H; case_eq (nth_error A B); intros
-                     | [ H : _ /\ _ |- _ ] => destruct H; clear H
-                     | [ H : Some _ = Some _ |- _ ] => inversion H; clear H; subst
-                     | [ H : ?X , H' : ?X -> ?Y |- _ ] => 
-                       specialize (H' H)
-                   end.
-          admit.
-          admit.
-          admit.
-
-
-          (** write **)
-          revert sfuncs_evals. admit.
+        clear. induction ls. destruct 1.
+        intros. destruct H. subst. exists nil. simpl; eauto.
+        apply IHls in H. do 2 destruct H. subst; eauto. exists (a :: x0). simpl; eauto.
       Qed.
 
-    End plugin_correct.
+      (** This is all going to get put in a record **)
+      Hypothesis mem_satisfies_himp : forall cs P Q stn_st,
+        mem_satisfies cs P stn_st ->
+        ST.himp cs P Q ->
+        mem_satisfies cs Q stn_st.
+      Hypothesis mem_satisfies_pure : forall cs p P stn_st,
+        mem_satisfies cs (ST.star (ST.inj p) P) stn_st ->
+        interp cs p.
+(*
+      Variable split : stn_st -> stn_st -> stn_st -> Prop.
+      Hypothesis mem_satisfies_star : forall cs P Q stn_st,
+        mem_satisfies cs (ST.star P Q) stn_st <->
+        exists ss1 ss2,
+          split stn_st ss1 ss2 /\
+          mem_satisfies cs P ss1 /\
+          mem_satisfies cs Q ss2.
+      Hypothesis mem_split_read : forall s s1 s2,
+        split s s1 s2 ->
+          forall p v,
+          ReadWord s1 p = Some v ->
+          ReadWord s p = Some v.
+      Hypothesis mem_split_write : forall s s1 s1' s2,
+        split s s1 s2 ->
+          forall p v,
+            WriteWord s1 p v = Some s1' ->
+            exists s', WriteWord s p v = Some s' /\
+            split s' s1' s2.
+*)
 
-    Ltac unfolder H :=
-      cbv delta 
-        [ fold_first fold_first_update 
-          FM.find FM.add 
-          plugin_symeval_read_word
-          plugin_symeval_write_word
-          MemEvaluator_plugin
-          smem_read smem_write 
-        ] in H.
+      Lemma pull_single : forall cs uvars vars SH x x1 x0 stn_st,
+        FM.find predIndex (SH.impures SH) = Some (x0 ++ x :: x1) ->
+        mem_satisfies cs (SEP.sexprD funcs preds uvars vars (SH.sheapD SH)) stn_st ->
+        mem_satisfies cs (SEP.sexprD funcs preds uvars vars
+          (SEP.Star (SEP.Func predIndex x) 
+            (SH.starred (SEP.Func predIndex) x0 (SH.starred (SEP.Func predIndex) x1
+              (SH.sheapD {| SH.impures := FM.remove predIndex (SH.impures SH)
+                ; SH.pures := SH.pures SH
+                ; SH.other := SH.other SH
+              |}))))) stn_st.
+      Proof.
+        intros. 
+        assert (SEP.heq funcs preds uvars vars cs 
+          (SH.sheapD SH) 
+          (SEP.Star (SEP.Func predIndex x) 
+            (SH.starred (SEP.Func predIndex) x0 (SH.starred (SEP.Func predIndex) x1
+              (SH.sheapD {| SH.impures := FM.remove predIndex (SH.impures SH)
+                ; SH.pures := SH.pures SH
+                ; SH.other := SH.other SH
+              |}))))).
+        { rewrite SH.starred_base. rewrite SH.starred_base.
+          repeat rewrite SH.sheapD_def. simpl. SF.heq_canceler.
+          rewrite SH.impuresD_Add with (f := predIndex) (argss := x0 ++ x :: x1).
+          rewrite SH.starred_def. rewrite fold_right_app. simpl.
+          rewrite <- SH.starred_def. rewrite SH.starred_base. rewrite <- SH.starred_def.
+          SF.heq_canceler. 
+          { unfold MM.PROPS.Add. intros. repeat (rewrite MM.FACTS.add_o || rewrite MM.FACTS.remove_o).
+            destruct (MF.FACTS.eq_dec predIndex y); subst; auto. }
+          { intro. apply MM.FACTS.remove_in_iff in H1. intuition; congruence. } }
+        eapply mem_satisfies_himp; eauto. apply SF.heq_himp; auto.
+      Qed.
 
-  End Plugin.
+      Theorem MemEvaluator_MemEvalPred_correct : @MemEvaluator_correct types pcT stT MemEvalPred_to_MemEvaluator
+        funcs preds stn_st ptrT valT mem_satisfies ReadWord WriteWord.
+      Proof.
+        constructor; simpl.
+        { intros. revert H. case_eq (FM.find predIndex (SH.impures SH)); try congruence; intros.
+          eapply fold_args_correct in H3. destruct H3. intuition.
+          apply in_split in H4. destruct H4. destruct H3. subst.
+          eapply pull_single in H; eauto.
+          simpl in *. rewrite predAt in H.
+          eapply sym_read_word_correct with (cs := cs) (Q := SEP.sexprD funcs preds uvars vars
+               (SH.starred (SEP.Func predIndex) x0
+                  (SH.starred (SEP.Func predIndex) x1
+                     (SH.sheapD
+                        {|
+                        SH.impures := FM.remove (elt:=
+                                        list (exprs types)) predIndex
+                                        (SH.impures SH);
+                        SH.pures := SH.pures SH;
+                        SH.other := SH.other SH |})))) in H5; eauto.
+          revert H. match goal with 
+                       | [ |- context [ match ?X with | _ => _ end ] ] => case_eq X
+                     end; intros; auto.
+          apply mem_satisfies_pure in H3. PropXTac.propxFo. }
+        { intros. revert H.
+          case_eq (FM.find predIndex (SH.impures SH)); try congruence.
+          do 2 intro.
+          case_eq (fold_args_update (fun args => pred_write_word mep P facts args pe ve) l); try congruence; intros.
+          inversion H5; clear H5; subst.
+          apply fold_args_update_correct in H4. do 4 destruct H4; intuition; subst.
+          eapply pull_single in H; eauto. simpl in H.
+          rewrite predAt in H.
+          eapply sym_write_word_correct with (cs := cs) 
+            (Q := (SEP.sexprD funcs preds uvars vars
+              (SH.starred (SEP.Func predIndex) x
+                 (SH.starred (SEP.Func predIndex) x0
+                    (SH.sheapD
+                       {|
+                       SH.impures := FM.remove (elt:=
+                                       list (exprs types)) predIndex
+                                       (SH.impures SH);
+                       SH.pures := SH.pures SH;
+                       SH.other := SH.other SH |}))))) 
+            in H4; eauto.
+          2: instantiate (1 := stn_m).
+          revert H4.
+          match goal with 
+            | [ |- match ?X with _ => _ end -> _ ] => 
+              case_eq X; try contradiction
+          end; intros.
+          revert H5. case_eq (WriteWord stn_m p v); try contradiction; intros.
+(*
+          eapply mem_satisfies_star in H6. do 2 destruct H6; intuition.
+
+          2: rewrite H4; eauto.
+          revert H5.
+          repeat match goal with
+                   | [ |- match ?X with _ => _ end -> _ ] =>
+                     case_eq X; intro; [ intro | contradiction ] 
+                 end; intros.
+          eapply mem_split_write in H8; eauto. destruct H8. intuition.
+          rewrite H11. 
+*)
+          eapply mem_satisfies_himp with (P := 
+            (SEP.sexprD funcs preds uvars vars
+              (SEP.Star (SEP.Func predIndex x2)
+            (SH.starred (SEP.Func predIndex) x
+               (SH.starred (SEP.Func predIndex) x0
+                  (SH.sheapD
+                     {|
+                     SH.impures := FM.remove (elt:=
+                                     list (exprs types)) predIndex
+                                     (SH.impures SH);
+                     SH.pures := SH.pures SH;
+                     SH.other := SH.other SH |})))))).
+          simpl. rewrite predAt. rewrite H4. eauto.
+          match goal with
+            | [ |- ST.himp ?cs (SEP.sexprD ?F ?P ?U ?G ?L) (SEP.sexprD _ _ _ _ ?R) ] =>
+              change (SEP.himp F P U G cs L R)
+          end.
+          apply SF.heq_himp. do 2 rewrite SH.starred_base.
+          repeat rewrite SH.sheapD_def; simpl. symmetry.
+          rewrite SH.impuresD_Add with (f := predIndex) (argss := x ++ x2 :: x0) (i := FM.remove predIndex (SH.impures SH)).
+          rewrite SH.starred_def. rewrite fold_right_app. simpl. rewrite <- SH.starred_def. rewrite SH.starred_base.
+          rewrite <- SH.starred_def. SF.heq_canceler.
+          { unfold MM.PROPS.Add. intros; repeat (rewrite MM.FACTS.add_o || rewrite MM.FACTS.remove_o).
+            destruct (MF.FACTS.eq_dec predIndex y); auto. }
+          { intro. apply MM.FACTS.remove_in_iff in H7; intuition congruence. }
+          revert H.
+          match goal with
+            | [ |- context [ match ?X with _ => _ end ] ] => 
+              case_eq X
+          end; intros; eauto.
+          apply mem_satisfies_pure in H5. PropXTac.propxFo. }
+      Qed.
+          
+    End To_MemEvaluator.
+
+  End PredEval.
 
   Module Composite.
     Section typed.
@@ -420,14 +547,14 @@ Module MemoryEvaluator (SH : SepHeap).
       Variable pcT stT : tvar.
 
       Definition MemEvaluator_composite (l r : MemEvaluator types pcT stT) : MemEvaluator types pcT stT :=
-        {| smemeval_read_word := fun P f e h => 
-           match smemeval_read_word l P f e h with
-             | None => smemeval_read_word r P f e h
+        {| sread_word := fun P f e h => 
+           match sread_word l P f e h with
+             | None => sread_word r P f e h
              | Some v => Some v
            end
-         ; smemeval_write_word := fun P f p v h => 
-           match smemeval_write_word l P f p v h with
-             | None => smemeval_write_word r P f p v h
+         ; swrite_word := fun P f p v h => 
+           match swrite_word l P f p v h with
+             | None => swrite_word r P f p v h
              | Some v => Some v
            end
          |}.
@@ -464,1311 +591,4 @@ Module MemoryEvaluator (SH : SepHeap).
     End typed.
   End Composite.
 
-End MemoryEvaluator.
-
-
-(*
-(* TODO: I want this to be a modularization of the plugin proofs *)
-Module Type PluginFacts (B : Heap) (ST : SepTheoryX.SepTheoryXType B).
-  Parameter Val : Type.
-
-  Parameter  smem_get_value : IL.settings -> B.addr -> ST.HT.smem -> 
-    option Val.
-  Parameter mem_get_value : IL.settings -> B.addr -> B.mem -> 
-    option Val.
-
-  Parameter smem_set_value : IL.settings -> B.addr -> Val
-    -> ST.HT.smem -> option ST.HT.smem.
-  Parameter mem_set_value : IL.settings -> B.addr -> Val
-    -> B.mem -> option B.mem.
-
-  Parameter smem_mem_get : forall stn p sm m v,
-    ST.HT.satisfies sm m ->
-    smem_get_value stn p sm = Some v ->
-    mem_get_value stn p m = Some v.
-
-  Parameter smem_mem_set : forall stn p v sm sm' m,
-    ST.HT.satisfies sm m ->
-    smem_set_value stn p v sm = Some sm' ->
-    exists m', 
-      mem_set_value stn p v m = Some m' /\
-      ST.HT.satisfies sm' m'.
-End PluginFacts.
-
-Module PluginWrap (B : Heap) (ST : SepTheoryX.SepTheoryXType B) (F : PluginFacts B ST) (PLUGIN : EvaluatorPluginType B ST).
-  Module Import SEP := PLUGIN.SEP.
-
-  Section typed.
-    Variable types : list type.
-
-    Variable tvState : tvar.
-    Variable tvPc : tvar.
-    Variable tvPtr : tvar.
-    Variable tvVal : tvar.
-    
-    Variable funcs : functions types.
-    Variable sfuncs : predicates types tvPc tvState.
-
-    Variable known : list nat.
-    Definition evals_type := 
-      hlist (fun n : nat => match nth_error sfuncs n with
-                              | None => Empty_set 
-                              | Some ss => @PLUGIN.SymEval types tvState tvPc tvPtr tvVal
-                                F.smem_get_value F.smem_set_value funcs ss
-                            end) known.
-
-    Variable evals : evals_type.
-
-    Definition symeval_read (hyps : list (expr types)) (p : expr types) 
-      (s : SEP.SHeap types tvPc tvState)
-      : option (expr types) :=
-      let hyps := hyps ++ pures s in
-      let reader ss seb args :=
-        PLUGIN.sym_read seb hyps args p
-      in
-      fold_known _ _ reader (impures s) evals.
-
-    Definition symeval_write (hyps : list (expr types)) (p v : expr types) 
-      (s : SEP.SHeap types tvPc tvState)
-      : option (SEP.SHeap types tvPc tvState) :=
-      let hyps := hyps ++ pures s in
-      let writer _ seb args := 
-        PLUGIN.sym_write seb hyps args p v
-      in
-      match fold_known_update _ _ writer (impures s) evals with
-        | None => None
-        | Some i' => Some {| impures := i' ; pures := pures s ; other := other s |}
-      end.
-
-  Lemma symeval_write_correct' : forall hyps pe ve s s',
-    symeval_write hyps pe ve s = Some s' ->
-    forall cs stn uvars vars m v,
-      AllProvable funcs uvars vars hyps ->
-      exprD funcs uvars vars ve tvPc = Some v ->
-      (exists sm, 
-           ST.satisfies cs (SEP.sexprD funcs sfuncs uvars vars (SH.sheapD s)) stn sm
-        /\ ST.HT.satisfies sm m) ->
-      match exprD funcs uvars vars pe tvPtr with
-        | Some p =>
-          exists m', 
-                F.mem_set_value types _ _ stn p v m = Some m'
-            /\ exists sm,
-               ST.satisfies cs (SEP.sexprD funcs sfuncs uvars vars (SH.sheapD s')) stn sm
-            /\ ST.HT.satisfies sm m'
-        | _ => False
-      end.
-  Proof.
-    unfold symeval_write. intros.
-    generalize dependent H.
-    match goal with
-      | [ |- context [ fold_known_update ?A ?B ?C ?D ?E ] ] =>
-        case_eq (fold_known_update A B C D E); intros; try congruence
-    end.
-    eapply fold_known_update_correct in H.
-    do 5 destruct H. destruct H2.
-    intuition. inversion H3; clear H3; subst. 
-        
-    eapply fold_args_update_correct in H6.
-    repeat match goal with
-             | [ H : exists x, _ |- _ ] => destruct H
-           end. intuition; subst.
-    generalize (SH.sheapD_pures _ _ _ _ _ H4).
-    rewrite SH.sheapD_pull_impure in H4 by eauto.
-    rewrite SEP.starred_In in H4.
-    rewrite <- SEP.heq_star_assoc in H4. rewrite SEP.heq_star_comm in H4.
-        
-    simpl in *. rewrite H2 in *.
-    intros.
-
-    eapply ST.satisfies_star in H4. do 2 destruct H4. intuition.
-
-    eapply PLUGIN.sym_write_correct with (stn := stn) (cs := cs) (m := x2)
-      in H3; eauto.
-
-    2: apply AllProvable_app; eauto.
-(*    
-    2: simpl in *;
-    match goal with
-      | [ |- context [ applyD ?A ?B ?C ?D ?E ] ] =>
-        destruct (applyD A B C D E); try solve [ intros; intuition | eapply ST.satisfies_pure in H4; PropXTac.propxFo ]
-    end.
-
-    destruct (exprD funcs uvars vars pe pcT); eauto.
-
-    repeat match goal with
-             | [ H : context [ match applyD ?A ?B ?C ?D ?E with
-                                 | Some _ => _
-                                 | None => _ 
-                               end ] |- _ ] =>
-               generalize dependent H; case_eq (applyD A B C D E); intros; intuition
-             | [ H : SepIL.ST.satisfies _ (SepIL.ST.inj _) _ _ |- _ ] =>
-               eapply SepIL.ST.satisfies_pure in H; PropXTac.propxFo; instantiate; intuition
-           end.
-    generalize dependent H8. case_eq (smem_write stn t v x2); intros; intuition.
-    
-    exists (SepIL.ST.HT.join s0 x3).
-    intuition.
-
-    rewrite SH.sheapD_pull_impure by eapply FM.find_add.
-    simpl. rewrite FM.remove_add.
-    eapply SepIL.ST.satisfies_star. do 2 eexists. split.
-
-    unfold tvarD in H4.
-
-    generalize dependent H3.
-    case_eq (SepIL.ST.HT.smem_set_word (IL.explode stn) a v x2); [ intros |
-      match goal with 
-        | [ |- context [ applyD ?A ?B ?C ?D ?E ] ] =>
-          destruct (applyD A B C D E); intros; exfalso; assumption
-      end ].
-        
-        exists (ST.HT.join s0 x3).
-        rewrite sheapD_pull_impure by eapply FM.find_add.
-        simpl. rewrite FM.remove_add.
-        rewrite starred_In.
-        simpl. rewrite H2. generalize dependent H8. 
-        rewrite <- ST.heq_star_assoc. rewrite ST.heq_star_comm. 
-        match goal with
-          | [ |- context [ applyD ?A ?B ?C ?D ?E ] ] =>
-            destruct (applyD A B C D E); try solve [ intros; intuition ]
-        end. 
-        generalize dependent H9.
-        match goal with
-          | [ |- ST.satisfies _ ?Y _ _ -> _ -> ST.satisfies _ (ST.star _ ?X) _ _ /\ _ ] => 
-            change X with Y; generalize dependent Y
-        end.
-        intros.
-
-        generalize (ST.HT.split_set_word _ _ (proj1 H7) _ _ _ _ H3).
-        split.
-        eapply ST.satisfies_star. do 2 eexists. split; eauto. eapply ST.HT.disjoint_split_join; eauto. tauto.
-
-        eapply ST.HT.satisfies_set_word. eauto. destruct H7; subst. tauto.
-
-        unfold tvarD. generalize dependent H4.
-        match goal with
-          | [ |- context [ applyD ?A ?B ?C ?D ?E ] ] =>
-            destruct (applyD A B C D E); try solve [ intros; intuition ]
-        end. intros.
-        eapply ST.satisfies_pure in H4. PropXTac.propxFo.
-      Qed.
-*)
-  Admitted.
-  End typed.
-End PluginWrap.
-
-Module PluginFacts_Word <: PluginFacts SepIL.BedrockHeap SepIL.ST.
-  Definition smem_get_value :=
-  
-End PluginFacts_Word.
-*)
-
-(*
-Module Evaluator (B : Heap) (ST : SepTheoryX.SepTheoryXType B).
-  Module Import SEP := SepExpr B ST.
-
-  Section typed.
-    Variable types' : list type.
-
-    Variable stateIndex : nat.
-    Variable pcIndex : nat.
-    Variable ptrIndex : nat.
-    Definition ptrType : type :=
-      {| Impl := B.addr
-       ; Eq := fun x y => match B.addr_dec x y with
-                           | left pf => Some pf
-                           | _ => None
-                         end
-       |}.
-
-    (** * Bytes *)
-    Section ByteAccess.
-      Variable byteIndex : nat.
-      Definition byteType : type :=
-        {| Impl := B
-         ; Eq := fun x y => match weq x y with
-                              | left pf => Some pf
-                              | _ => None
-                            end
-         |}.
-
-      Hypothesis byte_ptr : byteIndex <> ptrIndex.
-
-      Definition btypes := 
-        updatePosition ptrIndex ptrType (updatePosition byteIndex byteType types').
-
-      Variable funcs : functions btypes.
-
-      Lemma ptrType_get : tvarD btypes (tvType ptrIndex) = B.addr.
-        unfold btypes, tvarD. rewrite updatePosition_eq. reflexivity.
-      Qed.
-
-      Definition exprD_ptr (uvars vars : env btypes)
-        (e : expr btypes) : option B.addr :=
-        match ptrType_get in _ = t return option t with
-          | refl_equal => exprD funcs uvars vars e (tvType ptrIndex)
-        end.
-
-      Lemma byteType_get : tvarD btypes (tvType byteIndex) = B.
-        unfold btypes, tvarD. rewrite updatePosition_neq; auto;
-        rewrite updatePosition_eq; auto. congruence.
-      Qed.
-
-      Definition exprD_byte (uvars vars : env btypes)
-        (e : expr btypes) : option B :=
-        match byteType_get in _ = t return option t with
-          | refl_equal => exprD funcs uvars vars e (tvType byteIndex)
-        end.
-
-      Record SymEval_byte (Predicate : ssignature btypes (tvType pcIndex) (tvType stateIndex))
-        : Type :=
-      { sym_read_byte  : 
-        forall (hyps args : list (expr btypes)) (p : expr btypes), option (expr btypes)
-      ; sym_write_byte : 
-        forall (hyps args : list (expr btypes)) (p v : expr btypes),
-        option (list (expr btypes))
-      ; sym_read_byte_correct : forall args uvars vars cs hyps pe ve m stn,
-        sym_read_byte hyps args pe = Some ve ->
-        AllProvable funcs uvars vars hyps ->
-        match 
-          applyD (@exprD _ funcs uvars vars) (SDomain Predicate) args _ (SDenotation Predicate)
-          with
-          | None => False
-          | Some p => ST.satisfies cs p stn m
-        end ->
-        match exprD_ptr uvars vars pe , exprD_byte uvars vars ve with
-          | Some p , Some v =>
-            ST.HT.smem_get p m = Some v
-          | _ , _ => False
-        end
-      ; sym_write_byte_correct : forall args uvars vars cs hyps pe ve v m stn args',
-        sym_write_byte hyps args pe ve = Some args' ->
-        AllProvable funcs uvars vars hyps ->
-        exprD_byte uvars vars ve = Some v ->
-        match
-          applyD (@exprD _ funcs uvars vars) (SDomain Predicate) args _ (SDenotation Predicate)
-          with
-          | None => False
-          | Some p => ST.satisfies cs p stn m
-        end ->
-        match exprD_ptr uvars vars pe with
-          | Some p =>
-            match 
-              applyD (@exprD _ funcs uvars vars) (SDomain Predicate) args' _ (SDenotation Predicate)
-              with
-              | None => False
-              | Some pr => 
-                match ST.HT.smem_set p v m with
-                  | None => False
-                  | Some sm' =>
-                    ST.satisfies cs pr stn sm'
-                end
-            end
-          | _ => False
-        end
-      }.
-
-      Definition defaultSymEval_byte (P : ssignature btypes (tvType pcIndex) (tvType stateIndex))
-        : SymEval_byte P.
-      refine (
-        {| sym_read_byte          := fun _ _ _ => None
-         ; sym_write_byte         := fun _ _ _ _ => None
-         ; sym_read_byte_correct  := _
-         ; sym_write_byte_correct := _
-         |}); 
-      abstract (simpl; intros; congruence).
-      Defined.
-
-      Variable sfuncs : list (ssignature btypes (tvType pcIndex) (tvType stateIndex)).
-
-      Variable known : list nat. 
-      Variable evals : hlist (fun n : nat => match nth_error sfuncs n with
-                                               | None => Empty_set 
-                                               | Some ss => SymEval_byte ss
-                                             end) known.
-
-      Definition symeval_read_byte (hyps : list (expr btypes)) (p : expr btypes) 
-        (s : SHeap btypes (tvType pcIndex) (tvType stateIndex))
-        : option (expr btypes) :=
-        let hyps := hyps ++ pures s in
-        let reader _ seb args := 
-          sym_read_byte seb hyps args p
-        in
-        fold_known _ _  reader (impures s) evals.
-
-      Theorem symeval_read_byte_correct : forall cs stn hyps pe ve s uvars vars (m : B.mem),
-        symeval_read_byte hyps pe s = Some ve ->
-        AllProvable funcs uvars vars hyps ->
-        (exists sm, 
-          ST.satisfies cs (sexprD funcs sfuncs uvars vars (sheapD s)) stn sm
-          /\ ST.HT.satisfies sm m) ->
-        match exprD_ptr uvars vars pe , exprD_byte uvars vars ve with
-          | Some p , Some v => 
-            B.mem_get m p = Some v
-          | _ , _ => False
-        end.
-      Proof.
-        unfold symeval_read_byte. intros.
-        eapply fold_known_correct in H.
-        do 5 destruct H. destruct H1.
-        intuition.
-
-        generalize (sheapD_pures _ _ _ _ _ H); intros.
-
-        eapply sheapD_pull_impure 
-          with (funcs := funcs) (sfuncs := sfuncs) (a := uvars) (c := vars0) (cs := cs)
-            in H1.
-        apply In_split in H3. destruct H3. destruct H3.
-        subst. rewrite starred_In in H1.
-
-        rewrite <- heq_star_assoc in H1. rewrite heq_star_comm in H1.
-        rewrite H1 in H.
-        simpl in H.
-        eapply ST.satisfies_star in H. destruct H. destruct H. intuition.
-        rewrite H2 in *.
- 
-        eapply sym_read_byte_correct 
-          with (uvars := uvars) (vars := vars0) (cs := cs) (stn := stn) (m := x2)
-          in H6.
-        2: eapply AllProvable_app; auto.
-        destruct (exprD_ptr uvars vars0 pe); auto.
-        destruct (exprD_byte uvars vars0 ve); auto.
-        eapply ST.HT.satisfies_get. eauto.
-
-        eapply ST.HT.split_smem_get; eauto.
-        unfold tvarD.
-        match goal with 
-          | [ |- context [ applyD ?A ?B ?C ?D ?E ] ] =>
-            destruct (applyD A B C D E)
-        end; auto.
-        eapply ST.satisfies_pure in H. PropXTac.propxFo.
-      Qed.
-
-      Definition symeval_write_byte (hyps : list (expr btypes)) (p v : expr btypes) 
-        (s : SHeap btypes (tvType pcIndex) (tvType stateIndex))
-        : option (SHeap btypes (tvType pcIndex) (tvType stateIndex)) :=
-        let hyps := hyps ++ pures s in
-        let writer _ seb args := 
-          sym_write_byte seb hyps args p v
-        in
-        match fold_known_update _ _ writer (impures s) evals with
-          | None => None
-          | Some i' => Some {| impures := i' ; pures := pures s ; other := other s |}
-        end.
-
-      Theorem symeval_write_byte_correct : forall cs stn hyps pe ve v s s' uvars vars (m : B.mem),
-        symeval_write_byte hyps pe ve s = Some s' ->
-        AllProvable funcs uvars vars hyps ->
-        exprD_byte uvars vars ve = Some v ->
-        (exists sm, 
-             ST.satisfies cs (sexprD funcs sfuncs uvars vars (sheapD s)) stn sm
-          /\ ST.HT.satisfies sm m) ->
-        match exprD_ptr uvars vars pe with
-          | Some p =>
-            exists sm, 
-              ST.satisfies cs (sexprD funcs sfuncs uvars vars (sheapD s')) stn sm
-              /\ ST.HT.satisfies sm (B.mem_set m p v)
-          | _ => False
-        end.
-      Proof.
-        unfold symeval_write_byte. intros.
-        generalize dependent H.
-        match goal with
-          | [ |- context [ fold_known_update ?A ?B ?C ?D ?E ] ] =>
-            case_eq (fold_known_update A B C D E); intros; try congruence
-        end.
-        eapply fold_known_update_correct in H.
-        do 5 destruct H. destruct H2.
-        intuition. inversion H3; clear H3; subst. 
-        
-        eapply fold_args_update_correct in H6.
-        repeat match goal with
-                 | [ H : exists x, _ |- _ ] => destruct H
-               end. intuition; subst.
-        generalize (sheapD_pures _ _ _ _ _ H4).
-        rewrite sheapD_pull_impure in H4 by eauto.
-        rewrite starred_In in H4.
-        rewrite <- heq_star_assoc in H4. rewrite heq_star_comm in H4.
-        
-        simpl in *. rewrite H2 in *.
-        intros.
-
-        eapply ST.satisfies_star in H4. do 2 destruct H4. intuition.
-
-        eapply sym_write_byte_correct with (stn := stn) (cs := cs) (m := x2)
-          in H3; eauto.
-
-        2: apply AllProvable_app; eauto.
-
-        destruct (exprD_ptr uvars vars0 pe); eauto.
-        unfold tvarD in H3.
-
-        generalize dependent H3.
-        case_eq (ST.HT.smem_set a v x2); [ intros |
-          match goal with 
-            | [ |- context [ applyD ?A ?B ?C ?D ?E ] ] =>
-              destruct (applyD A B C D E); intros; exfalso; assumption
-          end ].
-        
-        exists (ST.HT.join s0 x3).
-        rewrite sheapD_pull_impure by eapply FM.find_add.
-        simpl. rewrite FM.remove_add.
-        rewrite starred_In.
-        simpl. rewrite H2. generalize dependent H8. 
-        rewrite <- ST.heq_star_assoc. rewrite ST.heq_star_comm. 
-        match goal with
-          | [ |- context [ applyD ?A ?B ?C ?D ?E ] ] =>
-            destruct (applyD A B C D E); try solve [ intros; intuition ]
-        end. 
-        generalize dependent H9.
-        match goal with
-          | [ |- ST.satisfies _ ?Y _ _ -> _ -> ST.satisfies _ (ST.star _ ?X) _ _ /\ _ ] => 
-            change X with Y; generalize dependent Y
-        end.
-        intros.
-
-        generalize (ST.HT.split_set _ _ (proj1 H7) _ _ _ H3).
-        split.
-        eapply ST.satisfies_star. do 2 eexists. split; eauto. eapply ST.HT.disjoint_split_join; eauto. tauto.
-
-        eapply ST.HT.satisfies_set. eauto. destruct H7; subst. tauto.
-
-        unfold tvarD. generalize dependent H4.
-        match goal with
-          | [ |- context [ applyD ?A ?B ?C ?D ?E ] ] =>
-            destruct (applyD A B C D E); try solve [ intros; intuition ]
-        end. intros.
-        eapply ST.satisfies_pure in H4. PropXTac.propxFo.
-      Qed.
-    End ByteAccess.
-
-    (** * Words *)
-    Section WordAccess.
-      Variable wordIndex : nat.
-      Definition wordType : type :=
-        {| Impl := W
-          ; Eq := fun x y => match weq x y with
-                               | left pf => Some pf
-                               | _ => None
-                             end
-        |}.
-
-      Hypothesis word_ptr : wordIndex <> ptrIndex.
-
-      Definition wtypes := 
-        updatePosition ptrIndex ptrType (updatePosition wordIndex wordType types').
-
-      Lemma ptrType_get_w : tvarD wtypes (tvType ptrIndex) = B.addr.
-        unfold wtypes, tvarD. rewrite updatePosition_eq. reflexivity.
-      Defined.
-
-      Definition exprD_ptr_w funcs (uvars vars : env wtypes)
-        (e : expr wtypes) : option B.addr :=
-        match ptrType_get_w in _ = t return option t with
-          | refl_equal => exprD funcs uvars vars e (tvType ptrIndex)
-        end.
-
-      Lemma wordType_get_w : tvarD wtypes (tvType wordIndex) = W.
-        unfold wtypes, tvarD. rewrite updatePosition_neq; auto;
-        rewrite updatePosition_eq; auto. congruence.
-      Defined.
-
-      Definition exprD_word funcs (uvars vars : env wtypes)
-        (e : expr wtypes) : option W :=
-        match wordType_get_w in _ = t return option t with
-          | refl_equal => exprD funcs uvars vars e (tvType wordIndex)
-        end.
-
-      Variable funcsT : functions wtypes -> functions wtypes.
-
-      Record SymEval_word (Predicate : ssignature wtypes (tvType pcIndex) (tvType stateIndex))
-        : Type :=
-      { sym_read_word  : 
-        forall (hyps args : list (expr wtypes)) (p : expr wtypes), option (expr wtypes)
-      ; sym_write_word : 
-        forall (hyps args : list (expr wtypes)) (p v : expr wtypes),
-        option (list (expr wtypes))
-      ; sym_read_word_correct : forall funcs args uvars vars cs hyps pe ve m stn,
-        sym_read_word hyps args pe = Some ve ->
-        AllProvable (funcsT funcs) uvars vars hyps ->
-        match 
-          applyD (exprD (funcsT funcs) uvars vars) (SDomain Predicate) args _ (SDenotation Predicate)
-          with
-          | None => False
-          | Some p => ST.satisfies cs p stn m
-        end ->
-        match 
-          exprD_ptr_w (funcsT funcs) uvars vars pe , 
-          exprD_word (funcsT funcs) uvars vars ve
-          with
-          | Some p , Some v =>
-            ST.HT.smem_get_word (IL.implode stn) p m = Some v
-          | _ , _ => False
-        end
-      ; sym_write_word_correct : forall funcs args uvars vars cs hyps pe ve v m stn args',
-        sym_write_word hyps args pe ve = Some args' ->
-        AllProvable (funcsT funcs) uvars vars hyps ->
-        exprD_word (funcsT funcs) uvars vars ve = Some v ->
-        match
-          applyD (@exprD _ (funcsT funcs) uvars vars) (SDomain Predicate) args _ (SDenotation Predicate)
-          with
-          | None => False
-          | Some p => ST.satisfies cs p stn m
-        end ->
-        match exprD_ptr_w (funcsT funcs) uvars vars pe with
-          | Some p =>
-            match 
-              applyD (@exprD _ (funcsT funcs) uvars vars) (SDomain Predicate) args' _ (SDenotation Predicate)
-              with
-              | None => False
-              | Some pr => 
-                match ST.HT.smem_set_word (IL.explode stn) p v m with
-                  | None => False
-                  | Some sm' => ST.satisfies cs pr stn sm'
-                end
-            end
-          | _ => False
-        end
-      }.
-
-      Definition defaultSymEval_word (P : ssignature wtypes (tvType pcIndex) (tvType stateIndex))
-        : SymEval_word P.
-      refine (
-        {| sym_read_word          := fun _ _ _ => None
-         ; sym_write_word         := fun _ _ _ _ => None
-         ; sym_read_word_correct  := _
-         ; sym_write_word_correct := _
-        |}); 
-      abstract (simpl; intros; congruence).
-      Defined.
-
-      (** * The full tactic *)
-      Variable sfuncs : list (ssignature wtypes (tvType pcIndex) (tvType stateIndex)).
-
-      Variable known : list nat. 
-      Variable evals : hlist (fun n : nat => match nth_error sfuncs n with
-                                               | None => Empty_set 
-                                               | Some ss => SymEval_word ss
-                                             end) known.
-
-      Definition symeval_read_word (hyps : list (expr wtypes)) (p : expr wtypes) 
-        (s : SHeap wtypes (tvType pcIndex) (tvType stateIndex))
-        : option (expr wtypes) :=
-        let hyps := hyps ++ pures s in
-        let reader ss (seb : SymEval_word ss) args := 
-          sym_read_word seb hyps args p
-        in
-        fold_known _ _ reader (impures s) evals.
-
-      Theorem symeval_read_word_correct : forall hyps pe s ve, 
-        symeval_read_word hyps pe s = Some ve ->
-        forall funcs cs stn uvars vars m,
-        AllProvable (funcsT funcs) uvars vars hyps ->
-        (exists sm, 
-             ST.satisfies cs (sexprD (funcsT funcs) sfuncs uvars vars (sheapD s)) stn sm
-          /\ ST.HT.satisfies sm m) ->
-        match 
-          exprD_ptr_w (funcsT funcs) uvars vars pe ,
-          exprD_word (funcsT funcs) uvars vars ve
-          with
-          | Some p , Some v => 
-            mem_get_word B.addr B.mem B.footprint_w B.mem_get (IL.implode stn) p m = Some v
-          | _ , _ => False
-        end.
-      Proof.
-        unfold symeval_read_word. intros.
-        eapply fold_known_correct in H.
-        do 5 destruct H. destruct H1.
-        intuition.
-
-        generalize (sheapD_pures _ _ _ _ _ H); intros.
-
-        eapply sheapD_pull_impure 
-          with (sfuncs := sfuncs) (a := uvars) (c := vars0) (cs := cs)
-            in H1.
-        apply In_split in H3. destruct H3. destruct H3.
-        subst. rewrite starred_In in H1.
-
-        rewrite <- heq_star_assoc in H1. rewrite heq_star_comm in H1.
-        rewrite H1 in H.
-        simpl in H.
-        eapply ST.satisfies_star in H. destruct H. destruct H. intuition.
-        rewrite H2 in *.
- 
-        eapply sym_read_word_correct 
-          with (uvars := uvars) (vars := vars0) (cs := cs) (stn := stn) (m := x2)
-          in H6.
-        2: eapply AllProvable_app; eauto.
-        destruct (exprD_ptr_w (funcsT funcs) uvars vars0 pe); auto.
-        destruct (exprD_word (funcsT funcs) uvars vars0 ve); auto.
-        eapply ST.HT.satisfies_get_word. eauto.
-
-        eapply ST.HT.split_smem_get_word; eauto.
-        unfold tvarD.
-        match goal with 
-          | [ |- context [ applyD ?A ?B ?C ?D ?E ] ] =>
-            destruct (applyD A B C D E)
-        end; auto.
-        eapply ST.satisfies_pure in H. PropXTac.propxFo.
-      Qed.
-
-      Definition symeval_write_word (hyps : list (expr wtypes)) (p v : expr wtypes) 
-        (s : SHeap wtypes (tvType pcIndex) (tvType stateIndex))
-        : option (SHeap wtypes (tvType pcIndex) (tvType stateIndex)) :=
-        let hyps := hyps ++ pures s in
-        let writer _ seb args := 
-          sym_write_word seb hyps args p v
-        in
-        match fold_known_update _ _ writer (impures s) evals with
-          | None => None
-          | Some i' => Some {| impures := i' ; pures := pures s ; other := other s |}
-        end.
-
-      Theorem symeval_write_word_correct : forall funcs hyps pe ve s s',
-        symeval_write_word hyps pe ve s = Some s' ->
-        forall cs stn uvars vars m v,
-        AllProvable (funcsT funcs) uvars vars hyps ->
-        exprD_word (funcsT funcs) uvars vars ve = Some v ->
-        (exists sm, 
-             ST.satisfies cs (sexprD (funcsT funcs) sfuncs uvars vars (sheapD s)) stn sm
-          /\ ST.HT.satisfies sm m) ->
-        match exprD_ptr_w (funcsT funcs) uvars vars pe with
-          | Some p =>
-            exists sm, 
-                 ST.satisfies cs (sexprD (funcsT funcs) sfuncs uvars vars (sheapD s')) stn sm
-              /\ ST.HT.satisfies sm (mem_set_word B.addr B.mem B.footprint_w B.mem_set (IL.explode stn) p v m)
-          | _ => False
-        end.
-      Proof.
-        unfold symeval_write_word. intros.
-        generalize dependent H.
-        match goal with
-          | [ |- context [ fold_known_update ?A ?B ?C ?D ?E ] ] =>
-            case_eq (fold_known_update A B C D E); intros; try congruence
-        end.
-        eapply fold_known_update_correct in H.
-        do 5 destruct H. destruct H2.
-        intuition. inversion H3; clear H3; subst. 
-        
-        eapply fold_args_update_correct in H6.
-        repeat match goal with
-                 | [ H : exists x, _ |- _ ] => destruct H
-               end. intuition; subst.
-        generalize (sheapD_pures _ _ _ _ _ H4).
-        rewrite sheapD_pull_impure in H4 by eauto.
-        rewrite starred_In in H4.
-        rewrite <- heq_star_assoc in H4. rewrite heq_star_comm in H4.
-        
-        simpl in *. rewrite H2 in *.
-        intros.
-
-        eapply ST.satisfies_star in H4. do 2 destruct H4. intuition.
-
-        eapply sym_write_word_correct with (stn := stn) (cs := cs) (m := x2)
-          in H3; eauto.
-
-        2: apply AllProvable_app; eauto.
-
-        destruct (exprD_ptr_w (funcsT funcs) uvars vars0 pe); eauto.
-        unfold tvarD in H3.
-
-        generalize dependent H3.
-        case_eq (ST.HT.smem_set_word (IL.explode stn) a v x2); [ intros |
-          match goal with 
-            | [ |- context [ applyD ?A ?B ?C ?D ?E ] ] =>
-              destruct (applyD A B C D E); intros; exfalso; assumption
-          end ].
-        
-        exists (ST.HT.join s0 x3).
-        rewrite sheapD_pull_impure by eapply FM.find_add.
-        simpl. rewrite FM.remove_add.
-        rewrite starred_In.
-        simpl. rewrite H2. generalize dependent H8. 
-        rewrite <- ST.heq_star_assoc. rewrite ST.heq_star_comm. 
-        match goal with
-          | [ |- context [ applyD ?A ?B ?C ?D ?E ] ] =>
-            destruct (applyD A B C D E); try solve [ intros; intuition ]
-        end. 
-        generalize dependent H9.
-        match goal with
-          | [ |- ST.satisfies _ ?Y _ _ -> _ -> ST.satisfies _ (ST.star _ ?X) _ _ /\ _ ] => 
-            change X with Y; generalize dependent Y
-        end.
-        intros.
-
-        generalize (ST.HT.split_set_word _ _ (proj1 H7) _ _ _ _ H3).
-        split.
-        eapply ST.satisfies_star. do 2 eexists. split; eauto. eapply ST.HT.disjoint_split_join; eauto. tauto.
-
-        eapply ST.HT.satisfies_set_word. eauto. destruct H7; subst. tauto.
-
-        unfold tvarD. generalize dependent H4.
-        match goal with
-          | [ |- context [ applyD ?A ?B ?C ?D ?E ] ] =>
-            destruct (applyD A B C D E); try solve [ intros; intuition ]
-        end. intros.
-        eapply ST.satisfies_pure in H4. PropXTac.propxFo.
-      Qed.
-
-    End WordAccess.
-  End typed.
-End Evaluator.
-*)
-(*
-Require Import SepIL SepTac.
-
-Module BedrockEvaluator_ptsto.
-  Module E := EvaluatorPlugin (BedrockHeap) (ST).
-
-  
-
-Module BedrockEvaluator.
-  Module E := EvaluatorPlugin (BedrockHeap) (ST).
-  Module Import SEP := E.SEP.
-
-  Definition pcIndex : nat := 0.
-  Definition stateIndex : nat := 1.
-  
-  Definition addr_type :=
-    {| Impl := W
-     ; Eq := seq_dec 
-     |}.
-
-  Definition word_type :=
-    {| Impl := W
-     ; Eq := seq_dec 
-     |}.
-
-  Definition wtypes := bedrock_types ++ addr_type :: word_type :: nil.
-
-  Definition ptsto32_ssig : ssignature wtypes (tvType pcIndex) (tvType stateIndex).
-  refine (
-  {| SepExpr.SDomain := tvType 2 :: tvType 3 :: nil
-   ; SepExpr.SDenotation := _
-   |}).
-  refine (ptsto32 _).
-  Defined.
-
-  Definition wordIndex := 3.
-  Definition ptrIndex := 2.
-  Lemma wordIndex_ptrIndex : wordIndex <> ptrIndex.
-    intro. inversion H.
-  Qed.
-
-  Variable funcs : functions wtypes.
-
-  (** TODO: maybe this should be like unification? 
-   ** - in that case the substitution is an effect and needs to be
-   **   threaded through the computation (monadically?)
-   **)
-  Variable expr_equal : forall (hyps : list (expr wtypes)) (tv : tvar) (a b : expr wtypes), bool.
-
-  Definition sym_read_word_ptsto32 (hyps args : list (expr wtypes)) (p : expr wtypes) 
-    : option (expr wtypes) :=
-    match args with
-      | p' :: v' :: nil => 
-        if expr_equal hyps (tvType ptrIndex) p p' then Some v' else None
-      | _ => None
-    end.
-  Definition sym_write_word_ptsto32 (hyps args : list (expr wtypes)) (p v : expr wtypes)
-    : option (list (expr wtypes)) :=
-    match args with
-      | p' :: v' :: nil =>
-        if expr_equal hyps (tvType ptrIndex) p p' then Some (p :: v :: nil) else None
-      | _ => None
-    end.
-
-  Variable expr_equal_correct : forall T hyps a b,
-    expr_equal hyps T a b = true ->
-    forall uvars vars,
-    AllProvable funcs uvars vars hyps ->
-    exprD funcs uvars vars a T = exprD funcs uvars vars b T.
-
-  Ltac expose :=
-    repeat (unfold wordIndex, ptrIndex in *; 
-            match goal with 
-              | [ H : match applyD _ _ ?A _ _ with
-                        | Some _ => _ 
-                        | None => False 
-                      end |- _ ] =>
-              destruct A; simpl in H; try (exfalso; assumption)
-              | [ H : match 
-                        match exprD ?A ?B ?C ?D ?E with
-                          | None => _
-                          | Some _ => _
-                        end _ _ 
-                        with 
-                        | None => _
-                        | Some _ => _
-                      end |- _ ] =>
-              generalize dependent H; case_eq (exprD A B C D E); simpl; intros; 
-                try (exfalso; assumption)
-              | [ H : context [ match expr_equal ?A ?B ?C ?D with
-                                  | true => _
-                                  | false => _
-                                end ] |- _ ] =>
-                generalize dependent H; case_eq (expr_equal A B C D); intros; 
-                  try (exfalso; congruence)
-              | [ H : expr_equal ?A ?B ?C ?D = true 
-                , H' : AllProvable _ _ _ ?A |- _ ] =>
-                generalize (@expr_equal_correct _ _ _ _ H _ _ H'); clear H; intros
-              | [ H : Some _ = Some _ |- _ ] =>
-                inversion H; clear H; subst
-              | [ H : exprD _ _ _ _ _ = Some _ |- _ ] =>
-                rewrite H in *
-            end; simpl in * ).
-
-  Lemma sym_read_word_ptsto32_correct : forall args uvars vars cs hyps pe ve m stn,
-    sym_read_word_ptsto32 hyps args pe = Some ve ->
-    AllProvable funcs uvars vars hyps ->
-    match 
-      applyD (exprD funcs uvars vars) (SDomain ptsto32_ssig) args _ (SDenotation ptsto32_ssig)
-      with
-      | None => False
-      | Some p => ST.satisfies cs p stn m
-    end ->
-    match exprD funcs uvars vars pe (tvType ptrIndex) , exprD funcs uvars vars ve (tvType wordIndex) with
-      | Some p , Some v =>
-        ST.HT.smem_get_word (IL.implode stn) p m = Some v
-      | _ , _ => False
-    end.
-  Proof.
-    simpl; intros; expose.
-    unfold ST.satisfies in H3. PropXTac.propxFo.
-  Qed.
-
-  Lemma sym_write_word_ptsto32_correct : forall args uvars vars cs hyps pe ve v m stn args',
-    sym_write_word_ptsto32 hyps args pe ve = Some args' ->
-    AllProvable funcs uvars vars hyps ->
-    exprD funcs uvars vars ve (tvType wordIndex) = Some v ->
-    match
-      applyD (@exprD _ funcs uvars vars) (SDomain ptsto32_ssig) args _ (SDenotation ptsto32_ssig)
-      with
-      | None => False
-      | Some p => ST.satisfies cs p stn m
-    end ->
-    match exprD funcs uvars vars pe (tvType ptrIndex)with
-      | Some p =>
-        match 
-          applyD (@exprD _ funcs uvars vars) (SDomain ptsto32_ssig) args' _ (SDenotation ptsto32_ssig)
-          with
-          | None => False
-          | Some pr => 
-            match ST.HT.smem_set_word (IL.explode stn) p v m with
-              | None => False
-              | Some sm' => ST.satisfies cs pr stn sm'
-            end
-        end
-      | _ => False
-    end.
-  Proof.
-    simpl; intros; expose.
-
-    unfold ST.satisfies in *. PropXTac.propxFo. 
-    case_eq (smem_set_word (IL.explode stn) t v m).
-    intros. unfold ptsto32. PropXTac.propxFo.
-    eapply smem_set_get_word_eq; eauto.
-    eapply IL.implode_explode.
-    eapply smem_set_get_valid_word; eauto.
-  Qed.
-
-  Definition SymEval_ptsto32 : E.SymEval_word wtypes wordIndex_ptrIndex funcs ptsto32_ssig :=
-    {| E.sym_read_word := sym_read_word_ptsto32 : list (expr (E.wtypes wtypes ptrIndex wordIndex)) -> _
-     ; E.sym_write_word := sym_write_word_ptsto32 
-     ; E.sym_read_word_correct := sym_read_word_ptsto32_correct
-     ; E.sym_write_word_correct := sym_write_word_ptsto32_correct
-     |}.
-
-End BedrockEvaluator.
-*)
-
-
-(** * These are generic search functions *)
-(*
-Section search_read_write.
-  Variable A : Type.
-  Variable B : A -> Type.
-  Variable types : list type.
-  Variable sfuncs : list A.
-
-  Variable T : Type.
-  Variable F : forall s, B s -> list (expr types) -> option T.
-  Variable F_upd : forall s, B s -> list (expr types) -> option (list (expr types)).
-
-  Section arg.
-    Variable ss : A.
-    Variable se : B ss.
-    
-    Fixpoint fold_args (es : list (list (expr types))) : option T :=
-      match es with 
-        | nil => None
-        | a :: b => 
-          match F se a with
-            | None => fold_args b
-            | Some r => Some r
-          end
-      end.
-    
-    Theorem fold_args_correct : forall es v,
-      fold_args es = Some v ->
-      exists k, In k es /\ F se k = Some v.
-    Proof.
-      clear. induction es.
-      simpl; congruence.
-      simpl. case_eq (F se a); intros.
-      inversion H0. subst. eauto.
-      eapply IHes in H0. destruct H0.
-      exists x. tauto.
-    Qed.
-
-    Fixpoint fold_args_update (es : list (list (expr types))) : option (list (list (expr types))) :=
-      match es with 
-        | nil => None
-        | a :: b => 
-          match F_upd se a with
-            | None => match fold_args_update b with
-                        | None => None
-                        | Some b => Some (a :: b)
-                      end
-            | Some r => Some (r :: b)
-          end
-      end.
-    
-    Theorem fold_args_update_correct : forall es es',
-      fold_args_update es = Some es' ->
-      exists pre, exists post, exists k, exists k',
-        es = pre ++ k :: post /\
-        F_upd se k = Some k' /\
-        es' = pre ++ k' :: post.
-    Proof.
-      clear. induction es.
-      simpl; congruence.
-      simpl. case_eq (F_upd se a); intros.
-      inversion H0. subst. do 4 eexists; intuition eauto.
-      instantiate (2 := nil). reflexivity. reflexivity.
-
-      generalize dependent H0.
-      case_eq (fold_args_update es); intros.
-      inversion H1; subst. eapply IHes in H0.
-      do 4 destruct H0. exists (a :: x). exists x0.
-      eexists; eexists; intuition; subst; eauto. reflexivity.
-
-      congruence.
-    Qed.
-  End arg.
-
-  Variable impures : FM.t (list (list (expr types))).
-
-  Fixpoint fold_known (k : list nat) :
-    hlist (fun n : nat => match nth_error sfuncs n return Type with
-                            | None => Empty_set 
-                            | Some ss => B ss
-                          end) k
-    -> option T :=
-    match k as k 
-      return hlist (fun n : nat => match nth_error sfuncs n return Type with
-                                     | None => Empty_set 
-                                     | Some ss => B ss
-                                   end) k
-      -> option T
-      with
-      | nil => fun _ => None
-      | a :: b => fun ss =>
-        match FM.find a impures with
-          | None => fold_known (hlist_tl ss)
-          | Some argss =>
-            match nth_error sfuncs a as ss
-              return match ss return Type with
-                       | None => Empty_set 
-                       | Some ss => B ss
-                     end -> option T
-              with
-              | Some _ => fun se =>
-                match fold_args se argss with
-                  | None => fold_known (hlist_tl ss)
-                  | Some r => Some r
-                end
-              | None => fun err => match err with end
-            end (hlist_hd ss)
-        end
-    end.
-  
-  Theorem fold_known_correct : forall k
-    (h : hlist (fun n : nat => match nth_error sfuncs n return Type with
-                                 | None => Empty_set 
-                                 | Some ss => B ss
-                               end) k) v,
-    @fold_known k h = Some v ->
-    exists n, exists ss,
-      exists se :  B ss, exists ls, exists args, 
-        nth_error sfuncs n = Some ss 
-        /\ FM.find n impures = Some ls 
-        /\ In args ls 
-        /\ F se args = Some v.
-  Proof.
-    clear. induction k; simpl.
-    congruence.
-    intros h v. specialize (IHk (hlist_tl h) v).
-    rewrite (hlist_eta _ h) in *.
-    generalize dependent (hlist_hd h). simpl.
-    case_eq (FM.find a impures); intros; eauto 10.
-
-    assert (exists k, nth_error sfuncs a = Some k).
-    generalize y. clear.
-    destruct (nth_error sfuncs a); [ eauto | destruct 1 ]. 
-    destruct H1.
-    generalize dependent y.
-    rewrite H1. intro.
-    case_eq (fold_args y l); intros; eauto 10.
-    inversion H2; subst.
-    eapply fold_args_correct in H0. destruct H0; eauto 10.
-  Qed.
-
-  Fixpoint fold_known_update (k : list nat) :
-    hlist (fun n : nat => match nth_error sfuncs n with
-                            | None => Empty_set 
-                            | Some ss => B ss
-                          end) k
-    -> option (FM.t (list (list (expr types)))) :=
-    match k as k 
-      return hlist (fun n : nat => match nth_error sfuncs n return Type with
-                                     | None => Empty_set 
-                                     | Some ss => B ss
-                                   end) k
-      -> option (FM.t (list (list (expr types))))
-      with
-      | nil => fun _ => None
-      | a :: b => fun ss =>
-        match FM.find a impures with
-          | None => fold_known_update (hlist_tl ss)
-          | Some argss =>
-            match nth_error sfuncs a as ss
-              return match ss return Type with
-                       | None => Empty_set 
-                       | Some ss => B ss
-                     end -> option (FM.t (list (list (expr types))))
-              with
-              | Some _ => fun se =>
-                match fold_args_update se argss with
-                  | None => fold_known_update (hlist_tl ss)
-                  | Some r => Some (FM.add a r impures) (* this is a replace *)
-                end
-              | None => fun err => match err with end
-            end (hlist_hd ss)
-        end
-    end.
-  
-  Theorem fold_known_update_correct : forall k
-    (h : hlist (fun n : nat => match nth_error sfuncs n return Type with
-                                 | None => Empty_set 
-                                 | Some ss => B ss
-                               end) k) i',
-    @fold_known_update k h = Some i' ->
-    exists n, exists ss,
-      exists se : B ss, exists ls, exists ls',
-        nth_error sfuncs n = Some ss 
-        /\ FM.find n impures = Some ls 
-        /\ fold_args_update se ls = Some ls'
-        /\ i' = FM.add n ls' impures.
-  Proof.
-    clear. induction k; simpl.
-    congruence.
-    intros h v. specialize (IHk (hlist_tl h) v).
-    rewrite (hlist_eta _ h) in *.
-    generalize dependent (hlist_hd h). simpl.
-    case_eq (FM.find a impures); intros; eauto 10.
-
-    assert (exists k, nth_error sfuncs a = Some k).
-    generalize y. clear.
-    destruct (nth_error sfuncs a); [ eauto | destruct 1 ]. 
-    destruct H1.
-    generalize dependent y.
-    rewrite H1. intro.
-    case_eq (fold_args_update y l); intros; eauto 10.
-    inversion H2; subst.
-    eauto 10.
-  Qed.
-
-End search_read_write.
-*)
-
-(*
-(** This depends on [IL.settings] 
- ** - this suggests that a better abstraction is to put the relevant settings into the
- **   memory model...
- **)
-Module Type EvaluatorPluginType (B : Heap) (ST : SepTheoryX.SepTheoryXType B).
-  Module SEP := SepExpr B ST.
-
-  Parameter MemEvalPred : list type -> Type.
-
-  Parameter smem_read : forall (types : list type),
-    @MemEvalPred types ->
-    forall (P : ProverT types),
-      Facts P -> exprs types -> expr types -> option (expr types).
-
-  Parameter smem_write : forall (types : list type),
-    @MemEvalPred types ->
-    forall (P : ProverT types), 
-      Facts P -> exprs types -> expr types -> expr types -> option (exprs types).
-
-  Parameter Build_MemEvalPred : forall (types : list type)
-    (sym_read : forall (P : ProverT types) (facts : Facts P) (args : list (expr types)) (p : expr types),
-      option (expr types))
-    (sym_write : forall (P : ProverT types) (facts : Facts P) (args : list (expr types)) (p v : expr types),
-      option (exprs types)),
-    @MemEvalPred types.
-
-  Parameter proj_sym_read : forall ts a b,
-    smem_read (types := ts) (Build_MemEvalPred a b) = a.
-
-  Parameter proj_sym_write : forall ts a b,
-    smem_write (types := ts) (Build_MemEvalPred a b) = b.
-
-  Parameter MemEvalPred_correct : forall
-    (types : list type) 
-    (me : MemEvalPred types)
- 
-    (tvState : tvar)
-    (tvPc : tvar)
-    (tvPtr : tvar)
-    (tvVal : tvar)
-      
-    (smem_get_value : IL.settings -> tvarD types tvPtr -> ST.HT.smem -> 
-      option (tvarD types tvVal))
-    (smem_set_value : IL.settings -> tvarD types tvPtr -> tvarD types tvVal
-      -> ST.HT.smem -> option ST.HT.smem)
-
-    (Predicate : SEP.ssignature types tvPc tvState),   
-    functions types -> Type.
-
-  Parameter sym_read_correct : forall
-    (types : list type)
-    (me : MemEvalPred types)
-    (tvState : tvar)
-    (tvPc : tvar)
-    (tvPtr : tvar)
-    (tvVal : tvar)
-      
-    (smem_get_value : IL.settings -> tvarD types tvPtr -> ST.HT.smem -> 
-      option (tvarD types tvVal))
-    (smem_set_value : IL.settings -> tvarD types tvPtr -> tvarD types tvVal
-      -> ST.HT.smem -> option ST.HT.smem)
-    
-    (Predicate : SEP.ssignature types tvPc tvState)
-    (funcs : functions types),
-    @MemEvalPred_correct types me tvState tvPc tvPtr tvVal smem_get_value smem_set_value Predicate funcs ->
-    forall P (PE : ProverT_correct P funcs),
-      forall args uvars vars cs facts pe p ve m stn,
-      smem_read me P facts args pe = Some ve ->
-      Valid PE uvars vars facts ->
-      exprD funcs uvars vars pe tvPtr = Some p ->
-      match 
-        applyD (exprD funcs uvars vars) (SDomain Predicate) args _ (SDenotation Predicate)
-        with
-        | None => False
-        | Some p => ST.satisfies cs p stn m
-      end ->
-      match exprD funcs uvars vars ve tvVal with
-        | Some v =>
-          smem_get_value stn p m = Some v
-        | _ => False
-      end.
-  
-  Parameter sym_write_correct : forall
-    (types : list type)
-    (me : MemEvalPred types)
-    (tvState : tvar)
-    (tvPc : tvar)
-    (tvPtr : tvar)
-    (tvVal : tvar)
-    
-    (smem_get_value : IL.settings -> tvarD types tvPtr -> ST.HT.smem -> 
-      option (tvarD types tvVal))
-    (smem_set_value : IL.settings -> tvarD types tvPtr -> tvarD types tvVal
-      -> ST.HT.smem -> option ST.HT.smem)
-    
-    (Predicate : SEP.ssignature types tvPc tvState)
-    (funcs : functions types),
-    @MemEvalPred_correct types me tvState tvPc tvPtr tvVal smem_get_value smem_set_value Predicate funcs ->
-    forall P (PE : ProverT_correct P funcs),
-      forall args uvars vars cs facts pe p ve v m stn args',
-      smem_write me P facts args pe ve = Some args' ->
-      Valid PE uvars vars facts ->
-      exprD funcs uvars vars pe tvPtr = Some p ->
-      exprD funcs uvars vars ve tvVal = Some v ->
-      match
-        applyD (@exprD _ funcs uvars vars) (SDomain Predicate) args _ (SDenotation Predicate)
-        with
-        | None => False
-        | Some p => ST.satisfies cs p stn m
-      end ->
-      match 
-        applyD (@exprD _ funcs uvars vars) (SDomain Predicate) args' _ (SDenotation Predicate)
-        with
-        | None => False
-        | Some pr => 
-          match smem_set_value stn p v m with
-            | None => False
-            | Some sm' => ST.satisfies cs pr stn sm'
-          end
-      end.
-
-  Parameter Build_MemEvalPred_correct : forall
-    (types : list type)
-    (me : MemEvalPred types)
-    (tvState : tvar)
-    (tvPc : tvar)
-    (tvPtr : tvar)
-    (tvVal : tvar)
-    
-    (smem_get_value : IL.settings -> tvarD types tvPtr -> ST.HT.smem -> 
-      option (tvarD types tvVal))
-    (smem_set_value : IL.settings -> tvarD types tvPtr -> tvarD types tvVal
-      -> ST.HT.smem -> option ST.HT.smem)
-    
-    (Predicate : SEP.ssignature types tvPc tvState)
-    (funcs : functions types)
-        
-    (sym_read_correct : forall P (PE : ProverT_correct P funcs),
-      forall args uvars vars cs facts pe p ve m stn,
-      smem_read me P facts args pe = Some ve ->
-      Valid PE uvars vars facts ->
-      exprD funcs uvars vars pe tvPtr = Some p ->
-      match 
-        applyD (exprD funcs uvars vars) (SDomain Predicate) args _ (SDenotation Predicate)
-        with
-        | None => False
-        | Some p => ST.satisfies cs p stn m
-      end ->
-      match exprD funcs uvars vars ve tvVal with
-        | Some v =>
-          smem_get_value stn p m = Some v
-        | _ => False
-      end)
-    (sym_write_correct : forall P (PE : ProverT_correct P funcs),
-      forall args uvars vars cs facts pe p ve v m stn args',
-      smem_write me P facts args pe ve = Some args' ->
-      Valid PE uvars vars facts ->
-      exprD funcs uvars vars pe tvPtr = Some p ->
-      exprD funcs uvars vars ve tvVal = Some v ->
-      match
-        applyD (@exprD _ funcs uvars vars) (SDomain Predicate) args _ (SDenotation Predicate)
-        with
-        | None => False
-        | Some p => ST.satisfies cs p stn m
-      end ->
-      match 
-        applyD (@exprD _ funcs uvars vars) (SDomain Predicate) args' _ (SDenotation Predicate)
-        with
-        | None => False
-        | Some pr => 
-          match smem_set_value stn p v m with
-            | None => False
-            | Some sm' => ST.satisfies cs pr stn sm'
-          end
-      end),
-    @MemEvalPred_correct types me tvState tvPc tvPtr tvVal smem_get_value smem_set_value Predicate funcs.
-
-End EvaluatorPluginType.
-*)
+End SymbolicEvaluator.
